% Preamble
\documentclass[11pt,reqno,oneside,a4paper]{article}
\usepackage[a4paper,includeheadfoot,left=25mm,right=25mm,top=00mm,bottom=20mm,headheight=20mm]{geometry}
\input{../texhead-main} % Standard packages, page layout, theorem environments, macros, etc
\input{../texhead-project} % Macros specific to this project.
\author{Wang Yanhua}
\title{Learning Langer's Method}
\renewcommand{\runningtitle}{Learning Langer's Method}
\date{\today}

\begin{document}
\maketitle
\thispagestyle{fancy}

\section{}

\begin{align*}
\cos(3x) &= \frac{1}{2}(e^{3ix} + e^{-3ix}) \iff\\
2e^{3ix} \cos(3x) &= (e^{6ix} + 1) \\
&= (1 \cdot (e^{6ix})^0  + 1 \cdot (e^{6ix})^1). \\
\intertext{By Langer's method,}
x &= \frac{1}{6i}\{2m \pi i + \log(-1)\} , (m=0, \pm 1, \pm 2, \cdots)\\
&= \frac{1}{6i}\{2m \pi i + i\pi\}\\
&=  \frac{1}{6}\{(2m+1)\pi\}.
\end{align*}

\section{}

As $\lim_{x \to \infty}   e^{-x} = 0 \text{ on the positive real axis}, \lim_{x \to \infty} \sin(x)+e^{-x} = \sin(x).$
\begin{align*}
\sin(x) &= \frac{1}{2i}(e^{ix}-e^{-ix}) \iff \\
2ie^{ix} (\sin(x)) &= (e^{2ix} - 1) \\
&=  (-1 \cdot (e^{2ix})^0 + 1 \cdot (e^{2ix})^1).\\
\intertext{By Langer's method,}
x &= \frac{1}{2i}\{2m \pi i + \log(1)\}  , (m=0, \pm 1, \pm 2, \cdots)\\
&= \frac{1}{2i}\{2m \pi i + 0\} \\
&= \{m \pi\}.
\end{align*}

\section{}

\begin{align*}
\sin(x) + \sinh(x) &= \frac{1}{2i}(e^{ix}-e^{-ix}) + \frac{1}{2}(e^x-e^{-x}).
\intertext{1st normal: } 
-2ie^{ix}(-\frac{1}{2i}e^{-ix} - \frac{1}{2}e^{-x})&=1 + ie^{ix-x}\\
&= ie^{(i-1)x} + 1.
\intertext{By Langer's method,}
x &= \frac{1}{i-1}\{2m \pi i + \log(i)\}  , (m=0, \pm 1, \pm 2, \cdots)\\
&= \frac{1}{i-1}\{2m \pi i + i\frac{\pi}{2}\}\\
&= \frac{1}{i-1}\{(2m+\frac{1}{2})i\pi\}.
\intertext{2nd normal: }
2ie^{ix}(-\frac{1}{2i}e^{-ix} + \frac{1}{2}e^{x}) &= -1 + ie^{ix+x}\\
&= ie^{(i+1)x} - 1.
\intertext{By Langer's method,}
x &= \frac{1}{i+1}\{2m \pi i + \log(-i)\}  , (m=0, \pm 1, \pm 2, \cdots)\\
&= \frac{1}{i+1}\{2m \pi i + i\frac{3\pi}{2}\}\\
&= \frac{1}{i+1}\{(2m+\frac{3}{2})i\pi\}.
\intertext{3rd normal: }
2ie^{-ix}(\frac{1}{2i}e^{ix} + \frac{1}{2}e^{x}) &= 1 + ie^{x-ix}\\
&= ie^{(1-i)x} + 1.
\intertext{By Langer's method,}
x &= \frac{1}{1-i}\{2m \pi i + \log(-i)\}  , (m=0, \pm 1, \pm 2, \cdots)\\
&= \frac{1}{1-i}\{2m \pi i + i\frac{3\pi}{2}\}\\
&= \frac{1}{1-i}\{(2m+\frac{3}{2})i\pi\}.
\intertext{4th normal: }
2ie^{-ix}(\frac{1}{2i}e^{ix} + \frac{1}{2}e^{x}) &= 1 + ie^{x-ix}\\
&= 1+ie^{(1-i)x}.
\intertext{By Langer's method,}
x &= \frac{1}{1-i}\{2m \pi i + \log(i)\}  , (m=0, \pm 1, \pm 2, \cdots)\\
&= \frac{1}{1-i}\{2m \pi i + i\frac{\pi}{2}\}\\
&= \frac{1}{1-i}\{(2m+\frac{1}{2})i\pi\}.
\end{align*}



\end{document}
